Weidenbach_Book/IsaSAT/IsaSAT_Show.thy
@@ -56,7 +56,7 @@ definition print_close_colour :: \<open>64 word \<Rightarrow> unit\<close> where
 
 definition isasat_current_information :: \<open>64 word \<Rightarrow> stats \<Rightarrow> clss_size \<Rightarrow> stats\<close> where
 \<open>isasat_current_information =
-   (\<lambda>curr_phase (propa, confl, decs, frestarts, lrestarts, uset, gcs, lbds) (lcount, lcountUE, lcountUS).
+   (\<lambda>curr_phase (propa, confl, decs, frestarts, lrestarts, uset, gcs, lbds) (lcount, lcountUE, lcountUS, _).
      if confl AND 8191 = 8191 \<comment> \<open>\<^term>\<open>8191 = 8192 - 1\<close>, i.e., we print when all first bits are 1.\<close>
      then do{
        let _ = print_c propa;
@@ -99,7 +99,7 @@ lemma isasat_current_status_id:
 
 definition isasat_print_progress :: \<open>64 word \<Rightarrow> 64 word \<Rightarrow> stats \<Rightarrow> clss_size \<Rightarrow> unit\<close> where
 \<open>isasat_print_progress c curr_phase =
-   (\<lambda>(propa, confl, decs, frestarts, lrestarts, uset, gcs, lbds) (lcount, lcountUE, lcountUS).
+   (\<lambda>(propa, confl, decs, frestarts, lrestarts, uset, gcs, lbds) (lcount, lcountUE, lcountUS, _).
      let
          _ = print_c propa;
          _ = if curr_phase = 1 then print_open_colour 33 else ();
